update

Auto/Embedding/LamBitVec.lean
@@ -17,7 +17,7 @@ namespace BitVec
   theorem eq_of_val_eq {a b : Std.BitVec n} (h : a.toNat = b.toNat) : a = b := by
     rcases a with ⟨⟨a, isLta⟩⟩; rcases b with ⟨⟨b, isLtb⟩⟩
     dsimp [Std.BitVec.toNat] at h; cases h; rfl
-    
+
   theorem val_eq_of_eq {a b : Std.BitVec n} (h : a = b) : a.toNat = b.toNat := by
     cases h; rfl
 
@@ -29,7 +29,7 @@ namespace BitVec
 
   theorem val_ne_of_ne {a b : Std.BitVec n} (h : a ≠ b) : a.toNat ≠ b.toNat := by
     intro h'; apply h; apply eq_of_val_eq h'
-  
+
   theorem ne_iff_val_ne {a b : Std.BitVec n} : a ≠ b ↔ a.toNat ≠ b.toNat :=
     Iff.intro val_ne_of_ne ne_of_val_ne
 
@@ -40,6 +40,10 @@ namespace BitVec
   theorem ushiftRight_def (a : Std.BitVec n) (i : Nat) : a >>> i = a.ushiftRight i := rfl
 
   theorem smtushiftRight_def (a : Std.BitVec n) (b : Std.BitVec m) : a >>> b = a >>> b.toNat := rfl
+
+  theorem neg_def (a : Std.BitVec n) : -a = a.neg := rfl
+
+  theorem sub_def (a b : Std.BitVec n) : a - b = a.sub b := rfl
 
   theorem toNat_shiftLeft {a : Std.BitVec n} (i : Nat) : (a <<< i).toNat = (a.toNat * (2 ^ i)) % (2 ^ n) := by
     rw [shiftLeft_def]; rcases a with ⟨⟨a, isLt⟩⟩
@@ -55,15 +59,39 @@ namespace BitVec
 
   theorem toNat_zeroExtend {a : Std.BitVec n} (i : Nat) : (a.zeroExtend i).toNat = a.toNat % (2 ^ i) := rfl
 
+  theorem toNat_sub (a b : Std.BitVec n) : (a - b).toNat = (a.toNat + (2 ^ n - b.toNat)) % (2 ^ n) := rfl
+
+  theorem toNat_neg (a : Std.BitVec n) : (-a).toNat = (2^n - a.toNat) % (2^n) := by
+    rw [neg_def]; dsimp [Std.BitVec.neg]
+    rw [← sub_def, toNat_sub, toNat_ofNat, Nat.zero_mod, Nat.zero_add]
+
   theorem shiftLeft_ge_length_eq_zero (a : Std.BitVec n) (i : Nat) : i ≥ n → a <<< i = 0#n := by
     intro h; apply eq_of_val_eq; rw [toNat_shiftLeft, toNat_ofNat]; apply Nat.mod_eq_zero_of_dvd
     have poweq : 2 ^ i = 2 ^ (i - n) * 2 ^ n := by rw [← Nat.pow_add, Nat.sub_add_cancel h]
     rw [poweq, ← Nat.mul_assoc, Nat.mul_comm _ (2^n)]; exact ⟨_, rfl⟩
 
-  theorem shiftRight_ge_length_eq_zero (a : Std.BitVec n) (i : Nat) : i ≥ n → a >>> i = 0#n := by
+  theorem ushiftRight_ge_length_eq_zero (a : Std.BitVec n) (i : Nat) : i ≥ n → a >>> i = 0#n := by
     intro h; apply eq_of_val_eq; rw [toNat_ushiftRight, toNat_ofNat]; apply (Nat.le_iff_div_eq_zero ?l).mpr ?r
     case l => apply Nat.pow_two_pos
     case r => apply Nat.le_trans (toNat_le _) (Nat.pow_le_pow_of_le_right (.step .refl) h)
+
+  theorem sshiftRight_ge_length_eq_msb (a : Std.BitVec n) (i : Nat) : i ≥ n → a.sshiftRight i =
+    if a.msb then (1#n).neg else 0#n := by
+    intro h; cases hmsb : a.msb <;> simp [sshiftRight, Std.BitVec.toInt, hmsb, Int.shiftRight_def]
+    case false => dsimp [Std.BitVec.ofInt]; apply ushiftRight_ge_length_eq_zero _ _ h
+    case true =>
+      rw [← Int.subNatNat_eq_coe, Int.subNatNat_of_lt (toNat_le _)]
+      simp [Std.BitVec.toInt, Std.BitVec.ofInt]
+      have hzero : Nat.pred (2 ^ n - Std.BitVec.toNat a) >>> i = 0 := by
+        rw [Nat.shiftRight_eq_div_pow]; apply (Nat.le_iff_div_eq_zero (Nat.pow_two_pos _)).mpr
+        rw [Nat.pred_lt_iff_le (Nat.pow_two_pos _)]
+        apply Nat.le_trans (Nat.sub_le _ _) (Nat.pow_le_pow_of_le_right (.step .refl) h)
+      rw [hzero, Nat.zero_mod, Nat.sub_zero]; apply eq_of_val_eq
+      rw [toNat_ofNat, ← neg_def, toNat_neg, toNat_ofNat]
+      cases n <;> try rfl
+      case succ =>
+        rw [Nat.mod_eq_of_lt (a:=1)]
+        apply @Nat.pow_le_pow_of_le_right 2 (.step .refl) 1 _ (Nat.succ_le_succ (Nat.zero_le _))
 
   theorem shiftRight_eq_zero_iff (a : Std.BitVec n) (b : Nat) : a >>> b = 0#n ↔ a.toNat < 2 ^ b := by
     rw [ushiftRight_def]; rcases a with ⟨⟨a, isLt⟩⟩; dsimp [ushiftRight, Std.BitVec.toNat]
@@ -82,11 +110,11 @@ namespace BitVec
   theorem ofNat_add (n a b : Nat) : (a + b)#n = a#n + b#n := by
     apply congrArg (f:=Std.BitVec.ofFin); apply Fin.eq_of_val_eq
     dsimp [Fin.ofNat']; rw [Nat.add_mod]; rfl
-  
+
   theorem ofNat_mod_pow2 (n a : Nat) : (a % (2 ^ n))#n = a#n := by
     apply congrArg (f:=Std.BitVec.ofFin); apply Fin.eq_of_val_eq
     dsimp [Fin.ofNat']; apply Nat.mod_mod
-  
+
   theorem ofNat_mul (n a b : Nat) : (a * b)#n = a#n * b#n := by
     apply congrArg (f:=Std.BitVec.ofFin); apply Fin.eq_of_val_eq
     dsimp [Fin.ofNat']; rw [Nat.mul_mod]; rfl
@@ -128,7 +156,30 @@ namespace BitVec
       have hne := of_decide_eq_false hdec
       rw [Bool.ite_eq_false _ _ _ (of_decide_eq_false hdec)]
       rw [smtushiftRight_def, eqof, shiftRight_eq_zero_iff] at hne
-      rw [shiftRight_ge_length_eq_zero]; rfl
+      rw [ushiftRight_ge_length_eq_zero]; rfl
+      apply Nat.le_trans (m:=2^n) (Nat.le_of_lt (Nat.le_pow (Nat.le_refl _)))
+      apply Nat.le_of_not_lt hne
+    case true =>
+      have heq := of_decide_eq_true hdec
+      rw [Bool.ite_eq_true _ _ _ heq]; apply congrArg
+      rw [smtushiftRight_def, eqof, shiftRight_eq_zero_iff] at heq
+      rw [toNat_zeroExtend, Nat.mod_eq_of_lt heq]
+
+  theorem sshr_equiv_short (a : Std.BitVec n) (b : Std.BitVec m) (h : m ≤ n) : a.sshiftRight b.toNat = a.sshiftRight (zeroExtend n b).toNat := by
+    apply eq_of_val_eq; rw [toNat_zeroExtend, Nat.mod_eq_of_lt]
+    apply Nat.le_trans (toNat_le _) (Nat.pow_le_pow_of_le_right (.step .refl) h)
+
+  theorem sshr_equiv_long (a : Std.BitVec n) (b : Std.BitVec m) (h : m > n) : a.sshiftRight b.toNat =
+    if (b >>> (n#m)) = 0#m then a.sshiftRight (zeroExtend n b).toNat else (if a.msb then (1#n).neg else 0#n) := by
+    have eqof : Std.BitVec.toNat n#m = n := by
+      rw [toNat_ofNat]; apply Nat.mod_eq_of_lt
+      apply Nat.le_trans (Nat.succ_le_succ (Nat.le_of_lt h)) (Nat.le_pow (Nat.le_refl _))
+    cases hdec : decide ((b >>> (n#m)) = 0#m)
+    case false =>
+      have hne := of_decide_eq_false hdec
+      rw [Bool.ite_eq_false _ _ _ (of_decide_eq_false hdec)]
+      rw [smtushiftRight_def, eqof, shiftRight_eq_zero_iff] at hne
+      rw [sshiftRight_ge_length_eq_msb]
       apply Nat.le_trans (m:=2^n) (Nat.le_of_lt (Nat.le_pow (Nat.le_refl _)))
       apply Nat.le_of_not_lt hne
     case true =>
@@ -199,9 +250,11 @@ def LamTerm.pushBVCast (ct : BVCastType) (t : LamTerm) : LamTerm :=
   | .none =>
     match t with
     | .lam s body => .lam s (pushBVCast .none body)
-    | .app _ (.base (.bvcst (.bvofNat n))) t' => pushBVCast (.ofNat n) t'
-    | .app _ (.base (.bvcst (.bvofInt n))) t' => pushBVCast (.ofInt n) t'
-    | .app s fn arg => .app s (pushBVCast .none fn) (pushBVCast .none arg)
+    | .app s fn arg =>
+      match fn with
+      | .base (.bvcst (.bvofNat n)) => pushBVCast (.ofNat n) arg
+      | .base (.bvcst (.bvofInt n)) => pushBVCast (.ofInt n) arg
+      | _ => .app s (pushBVCast .none fn) (pushBVCast .none arg)
     | _ => t
 
 theorem LamTerm.maxEVarSucc_pushBVCast : maxEVarSucc (pushBVCast ct t) = maxEVarSucc t := by
@@ -241,12 +294,14 @@ theorem LamTerm.maxEVarSucc_pushBVCast : maxEVarSucc (pushBVCast ct t) = maxEVar
                 rw [IH (t:=arg₁) (Nat.le_of_succ_le_succ (Nat.le_trans (Nat.le_trans
                   LamTerm.size_app_gt_size_arg LamTerm.size_app_ge_size_fn) tl))]
                 rw [IH (t:=arg) (Nat.le_of_succ_le_succ (Nat.le_trans
-                  LamTerm.size_app_gt_size_arg tl))])              
+                  LamTerm.size_app_gt_size_arg tl))])
       case ofInt m => apply Nat.max_zero_left
       case none =>
-        cases fn <;> try (
-          dsimp [maxEVarSucc, pushBVCast]; rw [IH (t:=arg) (Nat.le_of_succ_le_succ (
-            Nat.le_trans LamTerm.size_app_gt_size_arg tl))])
+        dsimp [pushBVCast]
+        have argeq : ∀ ct, maxEVarSucc (pushBVCast ct arg) = maxEVarSucc arg := by
+          intro ct; apply IH; apply Nat.le_of_succ_le_succ (Nat.le_trans _ tl)
+          apply LamTerm.size_app_gt_size_arg
+        cases fn <;> dsimp [maxEVarSucc] <;> (try rw [argeq])
         case base b =>
           cases b <;> try (
             dsimp [maxEVarSucc, pushBVCast]; rw [IH (t:=arg) (Nat.le_of_succ_le_succ (
